add assoc env plain bridge reductions

rocq/theories/TypeSystem/AssocEnvBridgeReductionFacts.v
@@ -1,6 +1,117 @@
 From Facet.TypeSystem Require Import
-  Lifetime Types Syntax Program TypingRules TypeChecker EnvStructuralRules AssocCompatibility
+  Lifetime Types Syntax Program TypingRules TypeChecker RootProvenance EnvStructuralRules
+  AssocCompatibility
   AssocCheckedBridgeReductionFacts AssocEnvStructural.
+From Stdlib Require Import List String.
+Import ListNotations.
+
+Inductive typed_args_env_structural_plain_witness
+    (env : global_env) (Ω : outlives_ctx) (n : nat)
+    : sctx -> list expr -> list param -> sctx -> Prop :=
+  | TESArgsPlainWitness_Nil : forall Σ,
+      typed_args_env_structural_plain_witness env Ω n Σ [] [] Σ
+  | TESArgsPlainWitness_Cons : forall Σ Σ1 Σ2 e es p ps T_e,
+      typed_env_structural env Ω n Σ e T_e Σ1 ->
+      ty_compatible Ω T_e (param_ty p) ->
+      typed_args_env_structural_plain_witness env Ω n Σ1 es ps Σ2 ->
+      typed_args_env_structural_plain_witness env Ω n Σ (e :: es) (p :: ps) Σ2.
+
+Inductive typed_args_roots_plain_witness
+    (env : global_env) (Ω : outlives_ctx) (n : nat)
+    : root_env -> sctx -> list expr -> list param ->
+      sctx -> root_env -> list root_set -> Prop :=
+  | TERArgsPlainWitness_Nil : forall R Σ,
+      typed_args_roots_plain_witness env Ω n R Σ [] [] Σ R []
+  | TERArgsPlainWitness_Cons : forall R R1 R2 Σ Σ1 Σ2 e es p ps T_e
+      roots roots_rest,
+      typed_env_roots env Ω n R Σ e T_e Σ1 R1 roots ->
+      ty_compatible Ω T_e (param_ty p) ->
+      typed_args_roots_plain_witness env Ω n R1 Σ1 es ps Σ2 R2 roots_rest ->
+      typed_args_roots_plain_witness env Ω n R Σ (e :: es) (p :: ps)
+        Σ2 R2 (roots :: roots_rest).
+
+Inductive typed_fields_env_structural_plain_witness
+    (env : global_env) (Ω : outlives_ctx) (n : nat)
+    : list lifetime -> list Ty -> sctx -> list (string * expr) ->
+      list field_def -> sctx -> Prop :=
+  | TESFieldsPlainWitness_Nil : forall lts args Σ fields,
+      typed_fields_env_structural_plain_witness env Ω n lts args Σ fields [] Σ
+  | TESFieldsPlainWitness_Cons : forall lts args Σ Σ1 Σ2 fields f rest
+      e_field T_field,
+      lookup_field_b (field_name f) fields = Some e_field ->
+      typed_env_structural env Ω n Σ e_field T_field Σ1 ->
+      ty_compatible Ω T_field (instantiate_struct_field_ty lts args f) ->
+      typed_fields_env_structural_plain_witness env Ω n lts args Σ1 fields
+        rest Σ2 ->
+      typed_fields_env_structural_plain_witness env Ω n lts args Σ fields
+        (f :: rest) Σ2.
+
+Inductive typed_fields_roots_plain_witness
+    (env : global_env) (Ω : outlives_ctx) (n : nat)
+    : list lifetime -> list Ty -> root_env -> sctx ->
+      list (string * expr) -> list field_def -> sctx -> root_env ->
+      root_set -> Prop :=
+  | TERFieldsPlainWitness_Nil : forall lts args R Σ fields,
+      typed_fields_roots_plain_witness env Ω n lts args R Σ fields [] Σ R []
+  | TERFieldsPlainWitness_Cons : forall lts args R R1 R2 Σ Σ1 Σ2 fields
+      f rest e_field T_field roots_field roots_rest,
+      lookup_field_b (field_name f) fields = Some e_field ->
+      typed_env_roots env Ω n R Σ e_field T_field Σ1 R1 roots_field ->
+      ty_compatible Ω T_field (instantiate_struct_field_ty lts args f) ->
+      typed_fields_roots_plain_witness env Ω n lts args R1 Σ1 fields rest
+        Σ2 R2 roots_rest ->
+      typed_fields_roots_plain_witness env Ω n lts args R Σ fields
+        (f :: rest) Σ2 R2 (root_set_union roots_field roots_rest).
+
+Lemma typed_args_env_structural_assoc_reduces_to_plain :
+  forall env Ω n Σ args ps Σ',
+    ty_compatible_assoc_checked_reduces_to_plain env Ω ->
+    typed_args_env_structural_assoc env Ω n Σ args ps Σ' ->
+    typed_args_env_structural_plain_witness env Ω n Σ args ps Σ'.
+Proof.
+  intros env Ω n Σ args ps Σ' Hcompat Hargs.
+  induction Hargs.
+  - constructor.
+  - econstructor; eauto.
+Qed.
+
+Lemma typed_args_roots_assoc_reduces_to_plain :
+  forall env Ω n R Σ args ps Σ' R' arg_roots,
+    ty_compatible_assoc_checked_reduces_to_plain env Ω ->
+    typed_args_roots_assoc env Ω n R Σ args ps Σ' R' arg_roots ->
+    typed_args_roots_plain_witness env Ω n R Σ args ps Σ' R' arg_roots.
+Proof.
+  intros env Ω n R Σ args ps Σ' R' arg_roots Hcompat Hargs.
+  induction Hargs.
+  - constructor.
+  - econstructor; eauto.
+Qed.
+
+Lemma typed_fields_env_structural_assoc_reduces_to_plain :
+  forall env Ω n lts args Σ fields defs Σ',
+    ty_compatible_assoc_checked_reduces_to_plain env Ω ->
+    typed_fields_env_structural_assoc env Ω n lts args Σ fields defs Σ' ->
+    typed_fields_env_structural_plain_witness env Ω n lts args Σ fields
+      defs Σ'.
+Proof.
+  intros env Ω n lts args Σ fields defs Σ' Hcompat Hfields.
+  induction Hfields.
+  - constructor.
+  - econstructor; eauto.
+Qed.
+
+Lemma typed_fields_roots_assoc_reduces_to_plain :
+  forall env Ω n lts args R Σ fields defs Σ' R' roots,
+    ty_compatible_assoc_checked_reduces_to_plain env Ω ->
+    typed_fields_roots_assoc env Ω n lts args R Σ fields defs Σ' R' roots ->
+    typed_fields_roots_plain_witness env Ω n lts args R Σ fields defs Σ' R'
+      roots.
+Proof.
+  intros env Ω n lts args R Σ fields defs Σ' R' roots Hcompat Hfields.
+  induction Hfields.
+  - constructor.
+  - econstructor; eauto.
+Qed.
 
 Lemma typed_args_env_structural_assoc_reduces_to_env_structural :
   forall env Ω n Σ args ps Σ',
